Using 2a,

\begin{align*}
  \Eps_1 \subseteq \sigma(\Eps_2) &\Rightarrow \sigma(\Eps_1) \subseteq \sigma(\sigma(\Eps_2)) \\
  &\Rightarrow \sigma(\Eps_1) \subseteq \sigma(\Eps_2) \\
\end{align*}

Similarly, 
\begin{align*}
  \Eps_2 \subseteq \sigma(\Eps_1) &\Rightarrow \sigma(\Eps_2) \subseteq \sigma(\sigma(\Eps_1)) \\
  &\Rightarrow \sigma(\Eps_2) \subseteq \sigma(\Eps_1) \\
\end{align*}

So, $\sigma(\Eps_1) \subseteq \sigma(\Eps_2)$ and 
$\sigma(\Eps_2) \subseteq \sigma(\Eps_1)$.

$\therefore~~ \sigma(\Eps_1) = \sigma(\Eps_2)$.
